As mentioned in the last Skype call, the [Term] datatype of L1g, L1_5, L2 and L3 now containg a constructor [TWrong], and compiling no longer returns option or exception.  THIS WILL BREAK SOMETHING IN L4, which I haven't fixed.
I made lots of other changes.  The only other change I think may be
observable to other levels of the compiler is that wcbvEval of L3
(both the relation and the function versions) is slightly more
liberal.  This change should not be observable for terms that come
from Coq.  (This is a time dependent claim, as Coq might change, and
the arbitrary internal representation that template-coq represents may
change.)

Updating before this commit, I had a good deal of frustration fixing
conflicts introduced by Matthieu (and a minor one by Abhishek).  Every
file in L3 had a conflict.  I realize Matthieu changed template-coq,
which naturally propogates through the whole compiler, but making the
changes for myself would leave me in better mood than fixing conflicts
and merges that didn't work in many files.

In future PLEASE DON'T CHANGE MY FILES WITHOUT FIRST EMAILING ME ABOUT
IT!!!.  Remember I am currently responsible for languages L1g, L1_5,
L2 and L3, which is a lot of files for conflicts.

theories/L2_typeStripped/compile.v
@@ -18,9 +18,9 @@ Set Implicit Arguments.
 Definition L1_5Term := L1_5.compile.Term.
 Definition L1_5Terms := L1_5.compile.Terms.
 Definition L1_5Defs := L1_5.compile.Defs.
-Definition L1_5Pgm := L1_5.compile.Program.
-Definition L1_5EC := @AstCommon.envClass L1_5Term.
-Definition L1_5Env := AstCommon.environ L1_5Term.
+Definition L1_5Pgm := Program L1_5Term.
+Definition L1_5EC := envClass L1_5Term.
+Definition L1_5Env := environ L1_5Term.
 
 
 Inductive Term : Type :=
@@ -33,11 +33,13 @@ Inductive Term : Type :=
 | TLetIn     : name -> Term -> Term -> Term
 | TApp       : Term -> Term (* first arg must exist *) -> Terms -> Term
 | TConst     : string -> Term
+| TAx        : Term
 | TInd       : inductive -> Term
-| TConstruct : inductive -> nat (* cnstr no *) -> Term
+| TConstruct : inductive -> nat (* cnstr no *) -> nat (* arity *) -> Term
 | TCase      : (inductive * nat * list nat) (* # parameters, # args per branch *) ->
                Term -> Terms -> Term
 | TFix       : Defs -> nat -> Term
+| TWrong     : Term
 with Terms : Type :=
 | tnil : Terms
 | tcons : Term -> Terms -> Terms
@@ -48,16 +50,12 @@ Hint Constructors Term Terms Defs.
 Scheme Trm_ind' := Induction for Term Sort Prop
   with Trms_ind' := Induction for Terms Sort Prop
   with Defs_ind' := Induction for Defs Sort Prop.
-Scheme Trm_ind2 := Induction for Term Sort Type
-  with Trms_ind2 := Induction for Terms Sort Type
-  with Defs_ind2 := Induction for Defs Sort Type.
 Combined Scheme TrmTrmsDefs_ind from Trm_ind', Trms_ind', Defs_ind'.
 Combined Scheme TrmTrms_ind from Trm_ind', Trms_ind'.
-Definition tunit (t:Term) : Terms := (tcons t tnil).
 Notation prop := (TSort SProp).
 Notation set_ := (TSort SSet).
 Notation type_ := (TSort SType).
-Notation x_ := (nAnon).
+Notation tunit t := (tcons t tnil).
 
 
 Function strip (t:L1_5Term) : Term :=
@@ -73,10 +71,12 @@ Function strip (t:L1_5Term) : Term :=
     | L1_5.compile.TApp fn arg args =>
       TApp (strip fn) (strip arg) (strips args)
     | L1_5.compile.TConst nm => TConst nm
+    | L1_5.compile.TAx => TAx
     | L1_5.compile.TInd i => TInd i
-    | L1_5.compile.TConstruct i m => TConstruct i m
+    | L1_5.compile.TConstruct i m arty => TConstruct i m arty
     | L1_5.compile.TCase n _ mch brs => TCase n (strip mch) (strips brs)
     | L1_5.compile.TFix ds n => TFix (stripDs ds) n
+    | L1_5.compile.TWrong => TWrong
   end
 with strips (ts:L1_5Terms) : Terms := 
   match ts with
@@ -91,32 +91,22 @@ with stripDs (ts:L1_5Defs) : Defs :=
 
 
 (** environments and programs **)
-Definition envClass := AstCommon.envClass Term.
-Definition environ := AstCommon.environ Term.
-Definition Program := AstCommon.Program Term.
-
-Function stripEC (ec:L1_5EC) : envClass :=
+Function stripEC (ec:L1_5EC) : AstCommon.envClass Term :=
   match ec with
-    | AstCommon.ecTrm t => AstCommon.ecTrm (strip t)
-    | AstCommon.ecTyp _ n itp => AstCommon.ecTyp Term n itp
+    | ecTrm t => ecTrm (strip t)
+    | ecTyp _ n itp => ecTyp Term n itp
   end.
 
-Definition  stripEnv : L1_5Env -> environ :=
+Definition  stripEnv : L1_5Env -> AstCommon.environ Term :=
   List.map (fun nmec : string * L1_5EC => (fst nmec, stripEC (snd nmec))).
 
-Definition stripProgram (p:L1_5Pgm) : Program :=
+Definition stripProgram (p:L1_5Pgm) : Program Term :=
   {| env:= stripEnv (env p);
      main:= strip (main p) |}.
 
-(*** from L0 to L2 ***)
-Definition program_Program (pgm:program) : exception Program :=
-  match L1_5.compile.program_Program pgm with
-    | Exc str => raise str
-    | Ret pgm => ret (stripProgram pgm)
-  end.
-Definition term_Term (t:term) : exception Term :=
-  match L1_5.compile.term_Term t with
-    | Exc str => raise str
-    | Ret trm => ret (strip trm)
-  end.
+(*** from L1 to L2 ***) 
+Definition program_Program (p:program) : Program Term :=
+  stripProgram (L1_5.compile.program_Program p).
 
+Definition term_Term (e:AstCommon.environ L1gTerm) (t:term) : Term :=
+  strip (L1_5.compile.term_Term e t).
